Working on a better way to do type casting.

Charge!/src/Charge/ModularFunc/ListType.v
@@ -28,8 +28,27 @@ Implicit Arguments ListTypeD [[typ] [RType_typ]].
 
 Section ListTypeD'.
   Context {typ : Type} {LT : ListType typ} {RType_typ : RType typ} {LTD : ListTypeD LT}.
+(*
+  Definition typD1 (t : typ) (f : typ -> typ) (g : Type -> Type) (p : typD (f t)) (e : typD (f t) = g (typD t)) : g (typD t)  :=
+    eq_rect _ id p _ e.
  
-  Definition listD (t : typ) (p : typD (tyList t)) : list (typD t) :=
+ Require Import Charge.ModularFunc.BaseType.
+ 
+  Definition typD2 (t u : typ) (f : typ -> typ -> typ) (g : Type -> Type -> Type) (p : typD (f t u)) (e : typD (f t u) = g (typD t) (typD u)) : g (typD t) (typD u) :=
+    eq_rect _ id p _ e.
+ 
+  Implicit Arguments typD1 [[t] [f] [g]].
+  Implicit Arguments typD2 [[t] [u] [f] [g]].
+ 
+  Definition listD (t : typ) (p : typD (tyList t)) : list (typD t) := typD1 p (btList t).
+  Context {BT : BaseType typ} {BTD : BaseTypeD}.
+  Definition pairD (t u : typ) (p : typD (tyProd t u)) : (typD t * typD u)%type := typD2 p (btProd t u).
+  
+  Program Definition test (a : typD (tyList (tyProd tyNat tyString))) : list (nat * string) := typD1 a _.
+  Proof.
+    apply typD1.
+ *)
+  Definition listD (t : typ) (p : typD (tyList t)) : list (typD t) := 
     eq_rect _ id p _ (btList t).
     
   Definition listR (t : typ) (p : list (typD t)) : typD (tyList t) :=
@@ -47,6 +66,45 @@ Section ListTypeD'.
     unfold listD, listR, eq_rect, eq_sym, id.
     destruct (btList t). reflexivity.
   Qed.
+  Require Import Charge.ModularFunc.BaseType.
+  Check stringD.
+Context {BT : BaseType typ} {BTD : BaseTypeD BT}.
+
+  Definition listE {A : Type} {t : typ} (e : typD t = A) : typD (tyList t) = list A :=
+    eq_ind (typD t) (fun B : Type => typD (tyList t) = list B) (btList t) A e.
+
+  Definition pairE {A B : Type} {t u : typ} (e1 : typD t = A) (e2 : typD u = B) : typD (tyProd t u) = (A * B)%type :=
+    eq_ind (typD t) (fun X : Type => typD (tyProd t u) = (X * B)%type)
+      (eq_ind (typD u) (fun Y : Type => typD (tyProd t u) = (typD t * Y)%type)
+         (btProd t u) B e2) A e1.
+
+  Definition trmD {A B : Type} (p : A) (e : A = B) : B :=
+    eq_rect _ id p _ e.
+    
+  Definition trmR {A B : Type} (p : B) (e : A = B) : A :=
+    eq_rect_r id p e.
+    
+    
+  Implicit Arguments trmD [[A] [B]].
+  Implicit Arguments trmR [[A] [B]].
+
+  Definition blurbel (lst : typD (tyList (tyProd tyNat tyString))) : list (nat * string) :=
+    trmD lst (listE (pairE btNat btString)).
+    
+  Definition trm
+
+  Definition listI {A : Type} {t : typ} (f : typD t -> A) (p : typD (tyList t)) : list A.
+  Proof.
+    pose proof (btList t).
+    rewrite H in p.
+    pose proof (cong (A := A)).
+    eq_rect _ id p _ (cong f (btList t)).
+    (eq_rect _ (fun t => f t) p _ (btList t)).
+  Print eq_rect.  
+  Definition pairI {A B : Type} {t u : typ} (f : typD t -> A) (g : typD u -> B) (p : typD (tyProd t u)) : A * B :=
+    let x := eq_rect _ id p _ (btProd t u) in (f (fst x), g (snd x)).
+  Definition blarbel (lst : typD (tyList (tyProd tyNat tyString))) : list (nat * String.string) :=
+    listI (pairI natD stringD) lst.
 
 End ListTypeD'.  
 
